examples/sess/proofs.v
@@ -137,7 +137,31 @@ wp_apply (GenConn.wp_send_fupdN (λ skI skR si, sess_own skI skR si rl p)
 iIntros "[??]"; iApply "post". by iFrame.
 Qed.
 
-Lemma wp_recv {TT : tele} skI skR rl cs
+Lemma wp_recv skI skR rl cs (m : iMsg Σ term) :
+  {{{ connected skI skR rl cs (<?> m) }}}
+    impl.recv (repr cs)
+  {{{ t' p, RET (repr t');
+      public t' ∗
+      connected skI skR rl cs p ∗
+      (public (si_key cs) ∨ iMsg_car m t' (Next p)) }}}.
+Proof.
+iIntros ""; iIntros (Φ) "[c own] post".
+rewrite /impl.recv. wp_pure _ credit:"c1". wp_pure _ credit:"c2".
+wp_pure _ credit:"c3". wp_apply wp_fupd.
+wp_apply (GenConn.wp_recv (λ skI skR si (t' : term),
+                           ∃ p, sess_own skI skR cs rl p ∗
+                                iMsg_car m t' (Next p))%I
+           with " [$c c1 c2 own]").
+{ iDestruct "own" as "[#fail|own]"; eauto.
+  iRight. iIntros (t' ts_send ts_recv) "inv".
+  iMod (sess_recv with "[$c1] own inv") as "[$ $]"; eauto. }
+iIntros "%t' (conn & #p_t' & inv)".
+iDestruct "inv" as "[#fail|(%p & own & inv)]"; eauto.
+{ iApply ("post" $! _ inhabitant). iFrame. by iFrame "#". }
+by iApply "post"; iFrame; eauto.
+Qed.
+
+Lemma wp_recv_tele {TT : tele} skI skR rl cs
   (t : TT → term) (P : TT → iProp) (p : TT → iProto Σ term) :
   {{{ connected skI skR rl cs (<?.. x> MSG t x {{ ▷ P x }}; p x) }}}
     impl.recv (repr cs)
@@ -153,7 +177,7 @@ wp_apply (GenConn.wp_recv (λ skI skR si (t' : term),
            with " [$c c1 c2 own]").
 { iDestruct "own" as "[#fail|own]"; eauto.
   iRight. iIntros (t' ts_send ts_recv) "inv".
-  iMod (sess_recv with "[$c1 $c2] own inv") as "[??]".
+  iMod (sess_recv_tele with "[$c1 $c2] own inv") as "[??]".
   iModIntro. by iFrame. }
 iIntros "%t' (conn & #p_t' & inv)". iApply "post". iFrame "#".
 iDestruct "inv" as "[#fail|inv]"; eauto. iRight.
@@ -180,7 +204,7 @@ wp_apply (GenConn.wp_recv (λ skI skR si (t' : term),
            with " [$c c1 c2 own]").
 { iDestruct "own" as "[#fail|own]"; eauto.
   iRight. iIntros (t' ts_send ts_recv) "inv".
-  iMod (sess_recv with "[$c1 $c2] own inv") as "[??]".
+  iMod (sess_recv_tele with "[$c1 $c2] own inv") as "[??]".
   iModIntro. by iFrame. }
 iIntros "%t' (conn & #p_t' & [#fail|inv])".
 { iApply ("post" $! t' inhabitant) . iFrame. by iFrame "#". }
@@ -209,7 +233,7 @@ wp_apply (GenConn.wp_recv (λ skI skR si (t : term),
              (<?.. x> MSG @tele_app TT _ (λ t, t) x {{ ▷ @tele_app TT _ (λ t, P t) x }};
                    @tele_app TT _ (λ t, p t) x)) with "[own]" as "own".
   { iApply (sess_own_le with "own"). rewrite /=. iModIntro. eauto. }
-  iMod (sess_recv with "[$c1 $c2] own inv") as "[? H]".
+  iMod (sess_recv_tele with "[$c1 $c2] own inv") as "[? H]".
   iModIntro. iFrame. iModIntro.
   iDestruct "H" as (x) "(-> & own & H)". rewrite /=. by iFrame. }
 iIntros "%t (conn & #p_t & [#fail|inv])".
